ContextBasicDenotation/theories/Notation.v
@@ -21,3 +21,7 @@ Notation WfWorldT := (WfWorld (V := value)) (only parsing).
 Notation FiberExtensionT := (fiber_extension (V := value)) (only parsing).
 Notation LogicQualifierT := (logic_qualifier (V := value)) (only parsing).
 Notation lstore_bound_part := (@lstore_bound_part value) (only parsing).
+
+Global Notation open_tm_env :=
+  (fun η e => map_fold (fun k x acc => open_tm k (vfvar x) acc) e η)
+  (only parsing).
